RocqOfRust/revm/revm_interpreter/interpreter/simulate/shared_memory.v
@@ -1,6 +1,12 @@
 Require Import simulate.RocqOfRust.
+Require Import core.simulate.option.
 Require Import core.num.simulate.mod.
 Require Import revm.revm_interpreter.interpreter.links.shared_memory.
+Require Import revm.revm_interpreter.links.gas.
+Require Import revm.revm_interpreter.links.interpreter.
+Require Import revm.revm_interpreter.links.interpreter_types.
+Require Import revm.revm_interpreter.simulate.gas.
+Require Import revm.revm_interpreter.simulate.interpreter_types.
 
 Definition num_words (len : usize) : usize :=
   Impl_usize.saturating_add len 31 /i 32.
@@ -17,3 +23,98 @@ Proof.
   }
   s.
 Qed.
+
+Definition resize_memory_cold
+    {Memory Synthetic Synthetic1 : Set}
+    `{Link Memory} `{Link Synthetic} `{Link Synthetic1}
+    {IMemoryTrait : MemoryTrait.C Memory Synthetic Synthetic1}
+    (gas : Gas.t)
+    (memory : Memory)
+    (new_num_words : usize) :
+    bool * (Gas.t * Memory) :=
+  let '(cost, memory_gas) :=
+    Impl_MemoryGas.record_new_len gas.(Gas.memory) new_num_words in
+  let gas := gas <| Gas.memory := memory_gas |> in
+  match cost with
+  | None =>
+    (false, (gas, memory))
+  | Some cost =>
+    match Impl_Gas.record_cost gas cost with
+    | None =>
+      (false, (gas, memory))
+    | Some gas =>
+      let '(_, memory) :=
+        IMemoryTrait.(MemoryTrait.resize) memory (new_num_words *i 32) in
+      (true, (gas, memory))
+    end
+  end.
+
+Definition resize_memory
+    {Memory Synthetic Synthetic1 : Set}
+    `{Link Memory} `{Link Synthetic} `{Link Synthetic1}
+    {IMemoryTrait : MemoryTrait.C Memory Synthetic Synthetic1}
+    (gas : Gas.t)
+    (memory : Memory)
+    (offset len : usize) :
+    bool * (Gas.t * Memory) :=
+  let new_num_words := num_words (Impl_usize.saturating_add offset len) in
+  if i[new_num_words] >? i[gas.(Gas.memory).(MemoryGas.words_num)] then
+    @resize_memory_cold
+      Memory Synthetic Synthetic1 H H0 H1 IMemoryTrait gas memory new_num_words
+  else
+    (true, (gas, memory)).
+
+Lemma resize_memory_eq
+    {WIRE : Set} `{Link WIRE}
+    {WIRE_types : InterpreterTypes.Types.t} `{InterpreterTypes.Types.AreLinks WIRE_types}
+    (run_InterpreterTypes_for_WIRE : InterpreterTypes.Run WIRE WIRE_types)
+    {IInterpreterTypes : InterpreterTypes.C WIRE_types}
+    (InterpreterTypesEq :
+      InterpreterTypes.Eq.t WIRE WIRE_types run_InterpreterTypes_for_WIRE IInterpreterTypes)
+    (interpreter : Interpreter.t WIRE WIRE_types)
+    (offset len : usize)
+    (stack : Stack.t) :
+  let ref_interpreter : '&mut (Interpreter.t WIRE WIRE_types) := make_ref 0 in
+  let ref_gas : '&mut Gas.t := {| Ref.core :=
+    SubPointer.Runner.apply
+      ref_interpreter.(Ref.core)
+      Interpreter.SubPointer.get_gas
+  |} in
+  let ref_memory : '&mut WIRE_types.(InterpreterTypes.Types.Memory) := {| Ref.core :=
+    SubPointer.Runner.apply
+      ref_interpreter.(Ref.core)
+      Interpreter.SubPointer.get_memory
+  |} in
+  let result :=
+    @resize_memory
+      WIRE_types.(InterpreterTypes.Types.Memory)
+      WIRE_types.(InterpreterTypes.Types.Memory_Synthetic)
+      WIRE_types.(InterpreterTypes.Types.Memory_Synthetic1)
+      H0.(InterpreterTypes.Types.H_Memory)
+      H0.(InterpreterTypes.Types.H_Memory_Synthetic)
+      H0.(InterpreterTypes.Types.H_Memory_Synthetic1)
+      IInterpreterTypes.(InterpreterTypes.MemoryTrait_for_Memory)
+      interpreter.(Interpreter.gas)
+      interpreter.(Interpreter.memory)
+      offset
+      len in
+  {{
+    SimulateM.eval_f
+      (run_resize_memory
+        run_InterpreterTypes_for_WIRE.(InterpreterTypes.run_MemoryTrait_for_Memory)
+        ref_gas
+        ref_memory
+        offset
+        len)
+      (interpreter :: stack)%stack 🌲
+    (
+      Output.Success (fst result),
+      (
+        interpreter
+          <| Interpreter.gas := fst (snd result) |>
+          <| Interpreter.memory := snd (snd result) |>
+        :: stack
+      )%stack
+    )
+  }}.
+Admitted.
